allow Map to pick its set instance for keyset and valueset -> now it works in RegAlloc
also refactor stuff to avoid importing potentially unwanted typeclass instances
by accident

bedrock2/src/NameGen.v
@@ -1,7 +1,5 @@
 Require Import Coq.Lists.List.
-Import ListNotations.
 Require Import compiler.util.Set.
-Require Export Coq.omega.Omega.
 
 Class NameGen(var st: Type){varsSet: SetFunctions var} := mkNameGen {
   (* Return a state which generates vars not contained in the given list.
@@ -25,56 +23,3 @@ Class NameGen(var st: Type){varsSet: SetFunctions var} := mkNameGen {
 
   freshNameGenState_spec: forall l v, In v l -> ~ v \in (allFreshVars (freshNameGenState l));
 }.
-
-Definition listmax(l: list nat): nat := fold_right max 0 l.
-
-Lemma listmax_spec: forall l v, In v l -> v <= listmax l.
-Proof.
-  induction l; intros.
-  - simpl in H. contradiction.
-  - simpl in *. destruct H.
-    + subst. apply Nat.le_max_l. 
-    + pose proof (Nat.le_max_r a (listmax l)).
-      specialize (IHl v H).
-      eapply Nat.le_trans; eassumption.
-Qed.
-
-Definition TODO{T: Type}: T. Admitted.
-
-Instance NatNameGen: NameGen nat nat := {|
-  freshNameGenState := fun l => S (listmax l);
-  genFresh := fun s => (s, S s);
-  (* allFreshVars := fun s => fun x => s <= x TODO can we still support infinite sets?? *)
-|}.
-  all: apply TODO. (*
-  abstract (intros; inversion H; subst; unfold subset; simpl; intuition omega).
-  abstract (unfold contains, Function_Set; intros; apply listmax_spec in H; omega).
-*)
-Defined.
-(* We use "abstract" to make the proofs opaque, but "Defined" to make sure that
-   "genFresh" and "allFreshVars" are transparent for reduction. *)
-
-
-Definition listmaxZ(l: list Z): Z := fold_right Z.max 0%Z l.
-
-Lemma listmaxZ_spec: forall l v, In v l -> (v <= listmaxZ l)%Z.
-Proof.
-  induction l; intros.
-  - simpl in H. contradiction.
-  - simpl in *. destruct H.
-    + subst. apply Z.le_max_l. 
-    + pose proof (Z.le_max_r a (listmaxZ l)).
-      specialize (IHl v H).
-      eapply Z.le_trans; eassumption.
-Qed.
-
-Instance ZNameGen: NameGen Z Z := {|
-  freshNameGenState := fun l => (listmaxZ l + 1)%Z;
-  genFresh := fun s => (s, (s + 1)%Z);
-(*  allFreshVars := fun s => fun x => (s <= x)%Z *)
-|}.
-  all: apply TODO. (*
-  abstract (intros; inversion H; subst; unfold subset; simpl; intuition omega).
-  abstract (unfold contains, Function_Set; intros; apply listmaxZ_spec in H; omega).
-*)
-Defined.
