bedrock2/src/util/Map.v
@@ -1,6 +1,5 @@
 Require Import compiler.util.Set.
 Require Import compiler.Decidable.
-Require Import Coq.Lists.List.
 
 Class MapFunctions(K V: Type) := mkMap {
   map: Type;
@@ -23,30 +22,3 @@ Class MapFunctions(K V: Type) := mkMap {
 }.
 
 Arguments map _ _ {_}.
-
-Definition TODO{T: Type}: T. Admitted.
-
-Instance List_Map(K V: Type)(domain_set: SetFunctions K)(range_set: SetFunctions V):
-  MapFunctions K V :=
-{|
-  map := list (K * V);
-  
-  map_domain_set := domain_set;
-  map_range_set := range_set;
-
-  empty_map := nil;
-  get A k := match find (fun a => if set_elem_eq_dec (fst a) k then true else false) A with
-             | Some (_, v) => Some v
-             | None => None
-             end;
-  put A k v := (fix rec A := match A with
-                            | (k1, v1) :: rest => if set_elem_eq_dec k1 k then (k, v) :: rest
-                                                 else (k1, v1) :: rec rest
-                            | nil => (k, v) :: nil
-                            end) A;
-  restrict M A := filter (fun p => containsb A (fst p)) M;
-  domain M := of_list (List.map fst M);
-  range M := of_list (List.map snd M);
-|}.
-all: apply TODO.
-Defined.
