bedrock2/src/util/Set.v
@@ -1,9 +1,7 @@
 Require Import compiler.util.Tactics.
 Require Import compiler.Decidable.
-Require Import compiler.util.ListLib.
 Require Import Coq.Program.Tactics.
-Require Import Coq.Lists.List.
-Import ListNotations.
+
 
 Class SetFunctions(E: Type) := mkSet {
   set: Type;
@@ -55,28 +53,6 @@ Section SetDefinitions.
 End SetDefinitions.
 
 Hint Unfold add subset disjoint : unf_set_defs.
-
-Definition TODO{T: Type}: T. Admitted.
-
-Instance List_Set(E: Type){eeq: DecidableEq E}: SetFunctions E := {|
-  set := list E;
-
-  contains A e := List.In e A;
-  containsb A e := if List.in_dec eeq e A then true else false;
-
-  empty_set := nil;
-  singleton_set e := (cons e nil);
-
-  union := list_union;
-  intersect := list_intersect;
-  diff := list_diff;
-  pick_or_else A default := match A with
-                             | a :: rest => (a, rest)
-                             | nil => (default, nil)
-                            end;
-|}.
-all: apply TODO.
-Defined.
 
 Ltac set_solver_generic E :=
   repeat autounfold with unf_set_defs in *;
