bedrock2/src/ZName.v
@@ -1,0 +1,4 @@
+Require Import Coq.ZArith.BinInt.
+Require Import compiler.NameWithEq.
+
+Instance ZName: NameWithEq := {| name := Z |}.
