bedrock2/src/ZNameGen.v
@@ -1,0 +1,44 @@
+Require Import Coq.Lists.List.
+Require Import Coq.omega.Omega.
+Require Import compiler.util.Set.
+Require Import compiler.util.List_Set.
+Require Import compiler.NameGen.
+
+Definition listmax(l: list nat): nat := fold_right max 0 l.
+
+Lemma listmax_spec: forall l v, In v l -> v <= listmax l.
+Proof.
+  induction l; intros.
+  - simpl in H. contradiction.
+  - simpl in *. destruct H.
+    + subst. apply Nat.le_max_l. 
+    + pose proof (Nat.le_max_r a (listmax l)).
+      specialize (IHl v H).
+      eapply Nat.le_trans; eassumption.
+Qed.
+
+Definition listmaxZ(l: list Z): Z := fold_right Z.max 0%Z l.
+
+Lemma listmaxZ_spec: forall l v, In v l -> (v <= listmaxZ l)%Z.
+Proof.
+  induction l; intros.
+  - simpl in H. contradiction.
+  - simpl in *. destruct H.
+    + subst. apply Z.le_max_l. 
+    + pose proof (Z.le_max_r a (listmaxZ l)).
+      specialize (IHl v H).
+      eapply Z.le_trans; eassumption.
+Qed.
+
+Definition TODO{T: Type}: T. Admitted.
+
+Instance ZNameGen: NameGen Z Z := {|
+  freshNameGenState := fun l => (listmaxZ l + 1)%Z;
+  genFresh := fun s => (s, (s + 1)%Z);
+(*  allFreshVars := fun s => fun x => (s <= x)%Z *)
+|}.
+  all: apply TODO. (*
+  abstract (intros; inversion H; subst; unfold subset; simpl; intuition omega).
+  abstract (unfold contains, Function_Set; intros; apply listmaxZ_spec in H; omega).
+*)
+Defined.
