bedrock2/src/examples/TestFlatImp.v
@@ -1,0 +1,66 @@
+Require Import riscv.util.BitWidths.
+Require Import compiler.util.Common.
+Require Import compiler.util.Tactics.
+Require Import compiler.Op.
+Require Import compiler.Memory.
+Require Import compiler.NameWithEq.
+Require Import riscv.util.BitWidth32.
+Require Import compiler.util.List_Map.
+Require Import compiler.util.List_Set.
+Require Import compiler.FlatImp.
+Require Import compiler.ZName.
+
+
+Definition var: Set := (@name ZName). (* only inside this test module *)
+
+Definition _n := 0%Z.
+Definition _a := 1%Z.
+Definition _b := 2%Z.
+Definition _s := 3%Z.
+Definition _one := 4%Z.
+(*
+one = 1
+n = input()
+a = 0
+b = 1
+loop:
+  stay in loop only if n nonzero
+  s = a+b
+  a = b
+  b = s
+  n = n - one
+ *)
+
+
+Example fib(n: word 32) :=
+  SSeq (SLit _one $1) (
+  SSeq (SLit _n n) (
+  SSeq (SLit _a $0) (
+  SSeq (SLit _b $1) (
+  SLoop SSkip
+        _n
+        (SSeq (SOp _s OPlus _a _b) (
+         SSeq (SSet _a _b) (
+         SSeq (SSet _b _s) (
+              (SOp _n OMinus _n _one)))))
+  )))).
+
+Definition annoying_eq: DecidableEq
+  (list (@name ZName) * list (@name ZName) * @stmt BitWidth32 ZName ZName). Admitted.
+Existing Instance annoying_eq.
+
+Definition eval_stmt_test fuel initialSt := @eval_stmt BitWidth32 ZName ZName _ (List_Map _ _) empty_map fuel initialSt no_mem.
+
+Example finalFibState(n: nat) := (eval_stmt_test 100 empty_map (fib $n)).
+Example finalFibVal(n: nat): option (word 32) := match finalFibState n with
+| Some (s, _) => get s _b
+| _ => None
+end.
+
+Goal finalFibVal 0 = Some $1. reflexivity. Qed.
+Goal finalFibVal 1 = Some $1. reflexivity. Qed.
+Goal finalFibVal 2 = Some $2. reflexivity. Qed.
+Goal finalFibVal 3 = Some $3. reflexivity. Qed.
+Goal finalFibVal 4 = Some $5. reflexivity. Qed.
+Goal finalFibVal 5 = Some $8. reflexivity. Qed.
+Goal finalFibVal 6 = Some $13. reflexivity. Qed.
