bedrock2/src/util/List_Map.v
@@ -1,0 +1,31 @@
+Require Import Coq.Lists.List.
+Require Import compiler.util.Set.
+Require Import compiler.Decidable.
+Require Import compiler.util.Map.
+Require Import compiler.util.List_Set.
+
+Definition TODO{T: Type}: T. Admitted.
+
+Instance List_Map(K V: Type){keq: DecidableEq K}{veq: DecidableEq V}: MapFunctions K V :=
+{|
+  map := list (K * V);
+  
+  map_domain_set := List_Set _;
+  map_range_set := List_Set _;
+
+  empty_map := nil;
+  get A k := match find (fun a => if set_elem_eq_dec (fst a) k then true else false) A with
+             | Some (_, v) => Some v
+             | None => None
+             end;
+  put A k v := (fix rec A := match A with
+                            | (k1, v1) :: rest => if set_elem_eq_dec k1 k then (k, v) :: rest
+                                                 else (k1, v1) :: rec rest
+                            | nil => (k, v) :: nil
+                            end) A;
+  restrict M A := filter (fun p => containsb A (fst p)) M;
+  domain M := of_list (List.map fst M);
+  range M := of_list (List.map snd M);
+|}.
+all: apply TODO.
+Defined.
